Add boolean

syntax.sig
@@ -2,3 +2,6 @@ tm : Type
 
 tAbs : (tm -> tm) -> tm
 tApp : tm -> tm -> tm
+tIf : tm -> tm -> tm -> tm
+tTrue : tm
+tFalse : tm
