theories/Autosubst2/syntax.v
@@ -6,12 +6,24 @@ Section tm.
 Inductive tm  : Type :=
   | var_tm : ( fin ) -> tm 
   | tAbs : ( tm   ) -> tm 
-  | tApp : ( tm   ) -> ( tm   ) -> tm .
+  | tApp : ( tm   ) -> ( tm   ) -> tm 
+  | tIf : ( tm   ) -> ( tm   ) -> ( tm   ) -> tm 
+  | tTrue : tm 
+  | tFalse : tm .
 
 Lemma congr_tAbs  { s0 : tm   } { t0 : tm   } (H1 : s0 = t0) : tAbs  s0 = tAbs  t0 .
 Proof. congruence. Qed.
 
 Lemma congr_tApp  { s0 : tm   } { s1 : tm   } { t0 : tm   } { t1 : tm   } (H1 : s0 = t0) (H2 : s1 = t1) : tApp  s0 s1 = tApp  t0 t1 .
+Proof. congruence. Qed.
+
+Lemma congr_tIf  { s0 : tm   } { s1 : tm   } { s2 : tm   } { t0 : tm   } { t1 : tm   } { t2 : tm   } (H1 : s0 = t0) (H2 : s1 = t1) (H3 : s2 = t2) : tIf  s0 s1 s2 = tIf  t0 t1 t2 .
+Proof. congruence. Qed.
+
+Lemma congr_tTrue  : tTrue  = tTrue  .
+Proof. congruence. Qed.
+
+Lemma congr_tFalse  : tFalse  = tFalse  .
 Proof. congruence. Qed.
 
 Definition upRen_tm_tm   (xi : ( fin ) -> fin) : ( fin ) -> fin :=
@@ -22,6 +34,9 @@ Fixpoint ren_tm   (xitm : ( fin ) -> fin) (s : tm ) : tm  :=
     | var_tm  s => (var_tm ) (xitm s)
     | tAbs  s0 => tAbs  ((ren_tm (upRen_tm_tm xitm)) s0)
     | tApp  s0 s1 => tApp  ((ren_tm xitm) s0) ((ren_tm xitm) s1)
+    | tIf  s0 s1 s2 => tIf  ((ren_tm xitm) s0) ((ren_tm xitm) s1) ((ren_tm xitm) s2)
+    | tTrue   => tTrue 
+    | tFalse   => tFalse 
     end.
 
 Definition up_tm_tm   (sigma : ( fin ) -> tm ) : ( fin ) -> tm  :=
@@ -32,6 +47,9 @@ Fixpoint subst_tm   (sigmatm : ( fin ) -> tm ) (s : tm ) : tm  :=
     | var_tm  s => sigmatm s
     | tAbs  s0 => tAbs  ((subst_tm (up_tm_tm sigmatm)) s0)
     | tApp  s0 s1 => tApp  ((subst_tm sigmatm) s0) ((subst_tm sigmatm) s1)
+    | tIf  s0 s1 s2 => tIf  ((subst_tm sigmatm) s0) ((subst_tm sigmatm) s1) ((subst_tm sigmatm) s2)
+    | tTrue   => tTrue 
+    | tFalse   => tFalse 
     end.
 
 Definition upId_tm_tm  (sigma : ( fin ) -> tm ) (Eq : forall x, sigma x = (var_tm ) x) : forall x, (up_tm_tm sigma) x = (var_tm ) x :=
@@ -45,6 +63,9 @@ Fixpoint idSubst_tm  (sigmatm : ( fin ) -> tm ) (Eqtm : forall x, sigmatm x = (v
     | var_tm  s => Eqtm s
     | tAbs  s0 => congr_tAbs ((idSubst_tm (up_tm_tm sigmatm) (upId_tm_tm (_) Eqtm)) s0)
     | tApp  s0 s1 => congr_tApp ((idSubst_tm sigmatm Eqtm) s0) ((idSubst_tm sigmatm Eqtm) s1)
+    | tIf  s0 s1 s2 => congr_tIf ((idSubst_tm sigmatm Eqtm) s0) ((idSubst_tm sigmatm Eqtm) s1) ((idSubst_tm sigmatm Eqtm) s2)
+    | tTrue   => congr_tTrue 
+    | tFalse   => congr_tFalse 
     end.
 
 Definition upExtRen_tm_tm   (xi : ( fin ) -> fin) (zeta : ( fin ) -> fin) (Eq : forall x, xi x = zeta x) : forall x, (upRen_tm_tm xi) x = (upRen_tm_tm zeta) x :=
@@ -58,6 +79,9 @@ Fixpoint extRen_tm   (xitm : ( fin ) -> fin) (zetatm : ( fin ) -> fin) (Eqtm : f
     | var_tm  s => (ap) (var_tm ) (Eqtm s)
     | tAbs  s0 => congr_tAbs ((extRen_tm (upRen_tm_tm xitm) (upRen_tm_tm zetatm) (upExtRen_tm_tm (_) (_) Eqtm)) s0)
     | tApp  s0 s1 => congr_tApp ((extRen_tm xitm zetatm Eqtm) s0) ((extRen_tm xitm zetatm Eqtm) s1)
+    | tIf  s0 s1 s2 => congr_tIf ((extRen_tm xitm zetatm Eqtm) s0) ((extRen_tm xitm zetatm Eqtm) s1) ((extRen_tm xitm zetatm Eqtm) s2)
+    | tTrue   => congr_tTrue 
+    | tFalse   => congr_tFalse 
     end.
 
 Definition upExt_tm_tm   (sigma : ( fin ) -> tm ) (tau : ( fin ) -> tm ) (Eq : forall x, sigma x = tau x) : forall x, (up_tm_tm sigma) x = (up_tm_tm tau) x :=
@@ -71,6 +95,9 @@ Fixpoint ext_tm   (sigmatm : ( fin ) -> tm ) (tautm : ( fin ) -> tm ) (Eqtm : fo
     | var_tm  s => Eqtm s
     | tAbs  s0 => congr_tAbs ((ext_tm (up_tm_tm sigmatm) (up_tm_tm tautm) (upExt_tm_tm (_) (_) Eqtm)) s0)
     | tApp  s0 s1 => congr_tApp ((ext_tm sigmatm tautm Eqtm) s0) ((ext_tm sigmatm tautm Eqtm) s1)
+    | tIf  s0 s1 s2 => congr_tIf ((ext_tm sigmatm tautm Eqtm) s0) ((ext_tm sigmatm tautm Eqtm) s1) ((ext_tm sigmatm tautm Eqtm) s2)
+    | tTrue   => congr_tTrue 
+    | tFalse   => congr_tFalse 
     end.
 
 Definition up_ren_ren_tm_tm    (xi : ( fin ) -> fin) (tau : ( fin ) -> fin) (theta : ( fin ) -> fin) (Eq : forall x, ((funcomp) tau xi) x = theta x) : forall x, ((funcomp) (upRen_tm_tm tau) (upRen_tm_tm xi)) x = (upRen_tm_tm theta) x :=
@@ -81,6 +108,9 @@ Fixpoint compRenRen_tm    (xitm : ( fin ) -> fin) (zetatm : ( fin ) -> fin) (rho
     | var_tm  s => (ap) (var_tm ) (Eqtm s)
     | tAbs  s0 => congr_tAbs ((compRenRen_tm (upRen_tm_tm xitm) (upRen_tm_tm zetatm) (upRen_tm_tm rhotm) (up_ren_ren (_) (_) (_) Eqtm)) s0)
     | tApp  s0 s1 => congr_tApp ((compRenRen_tm xitm zetatm rhotm Eqtm) s0) ((compRenRen_tm xitm zetatm rhotm Eqtm) s1)
+    | tIf  s0 s1 s2 => congr_tIf ((compRenRen_tm xitm zetatm rhotm Eqtm) s0) ((compRenRen_tm xitm zetatm rhotm Eqtm) s1) ((compRenRen_tm xitm zetatm rhotm Eqtm) s2)
+    | tTrue   => congr_tTrue 
+    | tFalse   => congr_tFalse 
     end.
 
 Definition up_ren_subst_tm_tm    (xi : ( fin ) -> fin) (tau : ( fin ) -> tm ) (theta : ( fin ) -> tm ) (Eq : forall x, ((funcomp) tau xi) x = theta x) : forall x, ((funcomp) (up_tm_tm tau) (upRen_tm_tm xi)) x = (up_tm_tm theta) x :=
@@ -94,6 +124,9 @@ Fixpoint compRenSubst_tm    (xitm : ( fin ) -> fin) (tautm : ( fin ) -> tm ) (th
     | var_tm  s => Eqtm s
     | tAbs  s0 => congr_tAbs ((compRenSubst_tm (upRen_tm_tm xitm) (up_tm_tm tautm) (up_tm_tm thetatm) (up_ren_subst_tm_tm (_) (_) (_) Eqtm)) s0)
     | tApp  s0 s1 => congr_tApp ((compRenSubst_tm xitm tautm thetatm Eqtm) s0) ((compRenSubst_tm xitm tautm thetatm Eqtm) s1)
+    | tIf  s0 s1 s2 => congr_tIf ((compRenSubst_tm xitm tautm thetatm Eqtm) s0) ((compRenSubst_tm xitm tautm thetatm Eqtm) s1) ((compRenSubst_tm xitm tautm thetatm Eqtm) s2)
+    | tTrue   => congr_tTrue 
+    | tFalse   => congr_tFalse 
     end.
 
 Definition up_subst_ren_tm_tm    (sigma : ( fin ) -> tm ) (zetatm : ( fin ) -> fin) (theta : ( fin ) -> tm ) (Eq : forall x, ((funcomp) (ren_tm zetatm) sigma) x = theta x) : forall x, ((funcomp) (ren_tm (upRen_tm_tm zetatm)) (up_tm_tm sigma)) x = (up_tm_tm theta) x :=
@@ -107,6 +140,9 @@ Fixpoint compSubstRen_tm    (sigmatm : ( fin ) -> tm ) (zetatm : ( fin ) -> fin)
     | var_tm  s => Eqtm s
     | tAbs  s0 => congr_tAbs ((compSubstRen_tm (up_tm_tm sigmatm) (upRen_tm_tm zetatm) (up_tm_tm thetatm) (up_subst_ren_tm_tm (_) (_) (_) Eqtm)) s0)
     | tApp  s0 s1 => congr_tApp ((compSubstRen_tm sigmatm zetatm thetatm Eqtm) s0) ((compSubstRen_tm sigmatm zetatm thetatm Eqtm) s1)
+    | tIf  s0 s1 s2 => congr_tIf ((compSubstRen_tm sigmatm zetatm thetatm Eqtm) s0) ((compSubstRen_tm sigmatm zetatm thetatm Eqtm) s1) ((compSubstRen_tm sigmatm zetatm thetatm Eqtm) s2)
+    | tTrue   => congr_tTrue 
+    | tFalse   => congr_tFalse 
     end.
 
 Definition up_subst_subst_tm_tm    (sigma : ( fin ) -> tm ) (tautm : ( fin ) -> tm ) (theta : ( fin ) -> tm ) (Eq : forall x, ((funcomp) (subst_tm tautm) sigma) x = theta x) : forall x, ((funcomp) (subst_tm (up_tm_tm tautm)) (up_tm_tm sigma)) x = (up_tm_tm theta) x :=
@@ -120,6 +156,9 @@ Fixpoint compSubstSubst_tm    (sigmatm : ( fin ) -> tm ) (tautm : ( fin ) -> tm 
     | var_tm  s => Eqtm s
     | tAbs  s0 => congr_tAbs ((compSubstSubst_tm (up_tm_tm sigmatm) (up_tm_tm tautm) (up_tm_tm thetatm) (up_subst_subst_tm_tm (_) (_) (_) Eqtm)) s0)
     | tApp  s0 s1 => congr_tApp ((compSubstSubst_tm sigmatm tautm thetatm Eqtm) s0) ((compSubstSubst_tm sigmatm tautm thetatm Eqtm) s1)
+    | tIf  s0 s1 s2 => congr_tIf ((compSubstSubst_tm sigmatm tautm thetatm Eqtm) s0) ((compSubstSubst_tm sigmatm tautm thetatm Eqtm) s1) ((compSubstSubst_tm sigmatm tautm thetatm Eqtm) s2)
+    | tTrue   => congr_tTrue 
+    | tFalse   => congr_tFalse 
     end.
 
 Definition rinstInst_up_tm_tm   (xi : ( fin ) -> fin) (sigma : ( fin ) -> tm ) (Eq : forall x, ((funcomp) (var_tm ) xi) x = sigma x) : forall x, ((funcomp) (var_tm ) (upRen_tm_tm xi)) x = (up_tm_tm sigma) x :=
@@ -133,6 +172,9 @@ Fixpoint rinst_inst_tm   (xitm : ( fin ) -> fin) (sigmatm : ( fin ) -> tm ) (Eqt
     | var_tm  s => Eqtm s
     | tAbs  s0 => congr_tAbs ((rinst_inst_tm (upRen_tm_tm xitm) (up_tm_tm sigmatm) (rinstInst_up_tm_tm (_) (_) Eqtm)) s0)
     | tApp  s0 s1 => congr_tApp ((rinst_inst_tm xitm sigmatm Eqtm) s0) ((rinst_inst_tm xitm sigmatm Eqtm) s1)
+    | tIf  s0 s1 s2 => congr_tIf ((rinst_inst_tm xitm sigmatm Eqtm) s0) ((rinst_inst_tm xitm sigmatm Eqtm) s1) ((rinst_inst_tm xitm sigmatm Eqtm) s2)
+    | tTrue   => congr_tTrue 
+    | tFalse   => congr_tFalse 
     end.
 
 Lemma rinstInst_tm   (xitm : ( fin ) -> fin) : ren_tm xitm = subst_tm ((funcomp) (var_tm ) xitm) .
@@ -175,6 +217,12 @@ Lemma renRen'_tm    (xitm : ( fin ) -> fin) (zetatm : ( fin ) -> fin) : (funcomp
 Proof. exact ((FunctionalExtensionality.functional_extensionality _ _ ) (fun n => renRen_tm xitm zetatm n)). Qed.
 
 End tm.
+
+
+
+
+
+
 
 
 
